

Switches

$$u(t) = \begin{cases} 0 & t < 0 \\ 1 & t > 0 \end{cases}$$

$$u(t-a) = \begin{cases} 0 & t < a \\ 1 & t > a \end{cases}$$

* This would be "off" until a !

$$\ddot{y} + 2\dot{y} + y = \underbrace{e^{-2t} + t^2}_{g(t)}$$

$$u(t-a)g(t)$$

In this case, we will start the forcing at a

Now, what if we wanted to turn a function off?

$$\overset{\text{turning on}}{(U(t-a) - \overset{\text{turning off}}{U(t-b)})g(t)}$$

$$\left\{ \begin{array}{ll} 0 & t < a \\ 1 & a < t < b \\ 0 & b < t \end{array} \right. \left. \begin{array}{l} \text{off until } a \\ \text{on from } a \text{ to } b \\ \text{off from } b \text{ until } \infty \end{array} \right\}$$

Second Shift Theorem

$$g(t)U(t-a) = e^{-as} \overset{\text{Laplace Transform}}{L[g(t+a)]}$$

$$\hookrightarrow U(t) \left\{ \begin{array}{ll} 0 & t < a \\ 1 & t > a \end{array} \right\}$$

$$f(t-a)U(t-a) = e^{-as} \overset{\text{Laplace Inverse}}{F(s)}$$

Example:

$$\begin{aligned}\mathcal{L}\{U(t-2)\} &= e^{-2s} \mathcal{L}\{g(t+2)\} \\ &= e^{-2s} \mathcal{L}\{t+2\} \\ &= e^{-2s} \left(\frac{1}{s^2} + \frac{2}{s} \right)\end{aligned}$$

Example:

$$\begin{aligned}\mathcal{L}\{t^2 U(t-3)\} &= e^{-3s} \mathcal{L}\{g(t+3)\} \\ &= e^{-3s} \mathcal{L}\{(t+3)^2\} \\ &= e^{-3s} \mathcal{L}\{t^2 + 6t + 9\} \\ &= e^{-3s} \left(\frac{2}{s^3} + \frac{6}{s^2} + \frac{9}{s} \right)\end{aligned}$$

Example

$$Y(s) = \frac{e^{-3s}}{s^2+1} = \underbrace{e^{-3s}}_{e^{-as}} \underbrace{\frac{1}{s^2+1}}_{F(s)}$$

$$F(s) = \frac{1}{s^2+1}$$

$$f(t) = \sin t$$

$$f(t-3)$$

$$\sin(t-3)U(t-3)$$

Example

$$\ddot{y} + 4\dot{y} + 4y = e^{-2t} + te^{-2t}$$

$$y(0) = 0, \quad \dot{y}(0) = 0$$

turns on at $t = 1$

turns off at $t = 3$

$$\ddot{y} + 4\dot{y} + 4y = \underbrace{(e^{-2t} + te^{-2t})}_{g(t)} [u(t-1) - u(t-3)]$$

$\downarrow \mathcal{L}$

$$s^2 Y(s) - \cancel{s y(0)}^0 - \cancel{\dot{y}(0)}^0 + 4(s Y(s) - \cancel{Y(0)}^0) + 4 Y(s) = \dots$$

$$Y(s)(s^2 + 4s + 4) = \mathcal{L}(f(t))$$
$$(s+2)^2$$

$$g(t) = e^{-2t} + te^{-2t}$$

$$u(t-1)g(t) - u(t-3)g(t)$$

* multiply the
switch out

$$U(t-1)g(t) - U(t-3)g(t) \quad \rightarrow \text{Later}$$

$$\downarrow$$

$$\mathcal{L}((e^{-2t} + te^{-2t})U(t-1))$$



* Using Second Shift theorem

$$\mathcal{L}\{g(t)U(t-a)\} = e^{-as} \mathcal{L}\{g(t+a)\}$$

$$= e^{-s} \mathcal{L}(g(e^{-2(t+1)} + (t+1)e^{-2(t+1)} - 1))$$

$$= e^{-s} \mathcal{L}(g(e^{-2t-2} + (t+1)e^{-2t-2}))$$

$$= e^{-s} \mathcal{L}(e^{-2t-2} (1 + (t+1)))$$

$$= e^{-s} \mathcal{L}(e^{-2t-2} (t+2))$$

$$= e^{-s} \mathcal{L}(e^{-2} e^{-2t} (t+2))$$

$$= e^{-s} e^{-2} \mathcal{L}(e^{-2t} (t+2))$$

$$= e^{-s} e^{-2} \mathcal{L}(te^{-2t} + 2e^{-2t}) = e^{-s} e^{-2} \left(\frac{1}{(s+2)^2} + 2\left(\frac{1}{s+2}\right) \right)$$

$$= e^{-s} e^{-2} \left(\frac{1}{(s+2)^2} + 2 \left(\frac{1}{s+2} \right) \right)$$

$$Y(s)(s+2)^2 = e^{-s} e^{-2} \left(\frac{1}{(s+2)^2} + 2 \left(\frac{1}{s+2} \right) \right) - \underbrace{e^{-3s} e^{-6} \left(\frac{1}{(s+2)^2} + \frac{4}{s+2} \right)}$$

From switch
close.
Same process